NonHamiltonian: Update

NonHamiltonian/Digraph.lean
@@ -25,67 +25,71 @@ structure Digraph where
   nodes          : NodeSet
   edges          : EdgeSet
   nodes_nonempty : nodes ≠ ∅ := by decide
-  edges_nodes    : edges.toList.all (λ (l,r) ↦
+  edges_endnodes : edges.toList.all (λ (l,r) ↦
     nodes.contains l && nodes.contains r) := by decide
   deriving Repr
 
 namespace Digraph
 
-theorem nodes_size_ne_zero (g : Digraph) : g.nodes.size ≠ 0 := by
+theorem nodes_size_ne_zero {g : Digraph} : g.nodes.size ≠ 0 := by
   simp [← g.nodes.eq_empty_iff_size_eq_zero, g.nodes_nonempty]
 
-theorem zero_lt_nodes_size (g : Digraph) : 0 < g.nodes.size := by
+theorem zero_lt_nodes_size {g : Digraph} : 0 < g.nodes.size := by
   rw [← Nat.ne_zero_iff_zero_lt]; exact g.nodes_size_ne_zero
 
-theorem edges_nodes' (g : Digraph) :
+theorem edges_endnodes' {g : Digraph} :
     ∀ e ∈ g.edges, e.1 ∈ g.nodes ∧ e.2 ∈ g.nodes := by
   simp only [← g.edges.mem_toList, ← g.nodes.contains_iff_mem,
-    ← Bool.and_eq_true]; exact List.all_eq_true.mp g.edges_nodes
+    ← Bool.and_eq_true]; exact List.all_eq_true.mp g.edges_endnodes
 
 /-! ## Hamiltonian Path -/
 
 structure HamiltonianPath (g : Digraph) where
-  path        : List Node
-  path_nodes  : path.all g.nodes.contains                 := by decide
-  nodes_path  : g.nodes.toList.all path.contains          := by decide
-  path_length : path.length = g.nodes.size                := by decide
-  path_edges  : (path.zip path.tail).all g.edges.contains := by decide
+  path      : List Node
+  path_perm : path.Perm g.nodes.toList := by decide
+  path_conn : path.connect.all g.edges.contains := by decide
+  deriving Repr, DecidableEq
 
 namespace HamiltonianPath
 
-theorem path_nonempty (g : Digraph) (p : HamiltonianPath g) :
+theorem path_length {g : Digraph} {p : HamiltonianPath g} :
+    p.path.length = g.nodes.size := by
+  rw [← g.nodes.length_toList]; exact List.Perm.length_eq p.path_perm
+
+theorem path_nonempty {g : Digraph} {p : HamiltonianPath g} :
     p.path ≠ [] := by
-  apply List.ne_nil_of_length_pos; rw [p.path_length]
+  apply List.ne_nil_of_length_pos; rw [path_length]
   exact g.zero_lt_nodes_size
 
-theorem path_nodes' (g : Digraph) (p : HamiltonianPath g) :
-    ∀ n ∈ p.path, n ∈ g.nodes := by
-  exact p.path.all_eq_true.mp p.path_nodes
-
-theorem nodes_path' (g : Digraph) (p : HamiltonianPath g) :
-    ∀ n ∈ g.nodes, n ∈ p.path := by
-  simp only [← g.nodes.mem_toList, ← p.path.contains_iff_mem]
-  exact List.all_eq_true.mp p.nodes_path
-
-theorem path_edges' (g : Digraph) (p :HamiltonianPath g) :
-    ∀ e ∈ p.path.zip p.path.tail, e ∈ g.edges := by
-  intro; apply List.all_eq_true.mp p.path_edges
+theorem path_conn_subset_edges {g : Digraph} {p :HamiltonianPath g} :
+    p.path.connect.Subset g.edges.toList := by
+  intro e; rw [g.edges.mem_toList]; exact List.all_eq_true.mp p.path_conn e
 
 end HamiltonianPath
 
-def hamiltonian (g : Digraph) : Prop :=
+def Hamiltonian (g : Digraph) : Prop :=
   Nonempty (HamiltonianPath g)
 
+/-- Tests whether digraph is Hamiltonian. -/
 def isHamiltonian (g : Digraph) : Bool :=
-  g.nodes.toList.perms.any (λ l ↦ (l.zip l.tail).all g.edges.contains)
+  g.nodes.toList.perms.any (·.connect.all g.edges.contains)
 
-theorem isHamiltonian_iff_hamiltonian (g : Digraph) :
-    g.isHamiltonian ↔ g.hamiltonian := by
-  constructor
-  · unfold isHamiltonian hamiltonian
-    intro h; simp at h
-    rcases h with ⟨hl, hr⟩
-    sorry
-  · sorry
+-- TODO: Relate this to isHamiltonian.
+def findHamiltonianPath? (g : Digraph) : Option (HamiltonianPath g) :=
+  Id.run do
+    for hperm : p in g.nodes.toList.perms do
+      if hconn : p.connect.all g.edges.contains then
+        return some ⟨p, List.perm_of_mem_perms hperm, hconn⟩
+    return none
+
+theorem isHamiltonian_iff_Hamiltonian {g : Digraph} :
+    g.isHamiltonian ↔ g.Hamiltonian := by
+  rw [isHamiltonian, List.any_eq_true, Hamiltonian]
+  constructor <;> rintro ⟨p, hperm, hconn⟩
+  · exact Nonempty.intro ⟨p, List.perm_of_mem_perms hperm, hconn⟩
+  · exists p; exact ⟨List.mem_perms_of_perm hperm, hconn⟩
+
+instance (g : Digraph) : Decidable (g.Hamiltonian) :=
+  decidable_of_iff (g.isHamiltonian) isHamiltonian_iff_Hamiltonian
 
 end Digraph
